Valid, coste de add

Auxiliary/Set.dfy
@@ -7,48 +7,60 @@ type Set< T(==) > {
 
   ghost function Universe():set<T>      // Upper bound del estado actual
 
+  ghost function Valid():bool
+  {
+    (Model() <= Universe()) &&
+    (|Model()| <= |Universe()|)
+  }
+
   ghost function Size():nat
     {|Universe()|*constant}
 
   method {:axiom} Pick(ghost counter_in:nat) returns (e:T, ghost counter_out:nat)
+    requires Valid()
     requires Model() != {}
-    ensures counter_out == counter_in + constant
     ensures e in Model()
     ensures e in Universe()
+    ensures counter_out == counter_in + constant
   
   method {:axiom} Empty(ghost counter_in:nat) returns (b:bool, ghost counter_out:nat)
+    requires Valid()
     ensures b == (Model() == {})
     ensures counter_out == counter_in + constant
   
   method {:axiom} Cardinality(ghost counter_in:nat) returns (size:int, ghost counter_out:nat)
+    requires Valid()
     ensures size == |Model()|
     ensures counter_out == counter_in + constant
   
+  method {:axiom} Contains(e:T, ghost counter_in:nat) returns (b:bool, ghost counter_out:nat)
+    requires Valid()
+    ensures  b == (e in Model()) 
+    ensures counter_out == counter_in + Size()
+  
   method {:axiom} Add(e:T, ghost counter_in:nat) returns (R:Set<T>, ghost counter_out:nat)
-    ensures R.Model() <= R.Universe()
-    ensures Universe() == Universe() + {e}
-    //requires e in Universe()
-    ensures  R.Model() == Model() + {e}
+    requires Valid()
+    ensures R.Valid()
+    ensures R.Universe() == Universe() + {e}
+    ensures R.Model() == Model() + {e}
     ensures if e in Model() then |R.Model()| == |Model()|
-            else |R.Model()| == |Model()| + constant
-    ensures counter_out == counter_in + constant
+            else |R.Model()| == |Model()| + 1
+    ensures counter_out == counter_in + Size()
 
   method {:axiom} Remove(e:T, ghost counter_in:nat) returns (R:Set<T>, ghost counter_out:nat)
-    ensures R.Model() <= R.Universe()
+    requires Valid()
+    ensures R.Valid()
     ensures R.Universe() == Universe()
     ensures  R.Model() == Model() - {e}
     ensures if e !in Model() then |R.Model()| == |Model()|
             else |R.Model()| == |Model()| - 1
     ensures counter_out == counter_in + Size()
   
-  method {:axiom} Contains(e:T, ghost counter_in:nat) returns (b:bool, ghost counter_out:nat)
-    ensures  b == (e in Model()) 
-    ensures counter_out == counter_in + Size()
-  
   method {:axiom} Copy(ghost counter_in:nat) returns (R:Set<T>, ghost counter_out:nat)
+    requires Valid()
+    ensures R.Valid()
     ensures R.Model() == Model()
     ensures R.Universe() == Model()
-    ensures R.Model() <= R.Universe()
     ensures counter_out == counter_in + Size()
 
 }
@@ -60,7 +72,12 @@ type SetSet< T(==) > {
   ghost function Model():set<set<T>>
 
   ghost function Universe():set<set<T>>
-  //ensures Model() <= Universe()
+
+  ghost function Valid():bool
+  {
+    (Model() <= Universe()) &&
+    (|Model()| <= |Universe()|)
+  }
 
   ghost function {:axiom} maximumSizeElements():nat
     ensures forall s | s in Universe() :: maximumSizeElements() >= |s|*constant
@@ -70,46 +87,53 @@ type SetSet< T(==) > {
     {|Universe()|*maximumSizeElements()}
 
   method {:axiom} Pick(ghost counter_in:nat) returns (e:Set<T>, ghost counter_out:nat)
+    requires Valid()
+    ensures e.Valid()
     requires Model() != {}
     ensures e.Size() <= maximumSizeElements()
     ensures e.Model() in Model()
     ensures counter_out == counter_in + maximumSizeElements()
 
   method {:axiom} Empty(ghost counter_in:nat) returns (b: bool, ghost counter_out:nat)
+    requires Valid()
     ensures b == (Model() == {})
     ensures counter_out == counter_in + constant
   
   method {:axiom} Cardinality(ghost counter_in:nat) returns (size: int, ghost counter_out:nat)
+    requires Valid()
     ensures size == |Model()|
     ensures counter_out == counter_in + constant
   
+  method {:axiom} Contains(e:Set<T>, ghost counter_in:nat) returns (b:bool, ghost counter_out:nat)
+    requires Valid()
+    ensures b == (e.Model() in Model()) 
+    ensures counter_out == counter_in + Size()
+  
   method {:axiom} Add(e:Set<T>, ghost counter_in:nat) returns (R:SetSet<T>, ghost counter_out:nat)
-    ensures R.Model() <= R.Universe()
+    requires Valid()
+    ensures R.Valid()
     ensures R.maximumSizeElements() == maximumSizeElements()
     ensures R.Universe() == Universe() + {e.Model()}
-    //requires e.Model() in Universe()
-    ensures  R.Model() == Model() + {e.Model()}
+    ensures R.Model() == Model() + {e.Model()}
     ensures if e.Model() in Model() then |R.Model()| == |Model()|
             else |R.Model()| == |Model()| + constant
-    ensures counter_out == counter_in + maximumSizeElements()
+    ensures counter_out == counter_in + Size()
 
   method {:axiom} Remove(e:Set<T>, ghost counter_in:nat) returns (R:SetSet<T>, ghost counter_out:nat)
-    ensures R.Model() <= R.Universe()
+    requires Valid()
+    ensures R.Valid()
     ensures R.Universe() == Universe()
     ensures R.maximumSizeElements() == maximumSizeElements()
-    ensures  R.Model() == Model() - {e.Model()}
+    ensures R.Model() == Model() - {e.Model()}
     ensures if e.Model() !in Model() then |R.Model()| == |Model()|
             else |R.Model()| == |Model()| - 1
     ensures counter_out == counter_in + Size()
-  
-  method {:axiom} Contains(e:Set<T>, ghost counter_in:nat) returns (b:bool, ghost counter_out:nat)
-    ensures  b == (e.Model() in Model()) 
-    ensures counter_out == counter_in + Size()
 
   method {:axiom} Copy(ghost counter_in:nat) returns (R:SetSet<T>, ghost counter_out:nat)
+    requires Valid()
+    ensures R.Valid()
     ensures R.Model() == Model()
     ensures R.Universe() == Model()
-    ensures R.Model() <= R.Universe()
     ensures R.maximumSizeElements() == maximumSizeElements()
     ensures counter_out == counter_in + Size()
 }
@@ -118,14 +142,21 @@ type SetSet< T(==) > {
 
 type SetSetSet< T(==) > {
 
-   ghost function Model():set<set<set<T>>>
-   ghost function Universe():set<set<set<T>>>
+  ghost function Model():set<set<set<T>>>
 
-   ghost function {:axiom} maximumSizeElements():nat
+  ghost function Universe():set<set<set<T>>>
+
+  ghost function Valid():bool
+  {
+    (Model() <= Universe()) &&
+    (|Model()| <= |Universe()|)
+  }
+
+  ghost function {:axiom} maximumSizeElements():nat
     ensures forall s | s in Universe() :: maximumSizeElements() >= |s|*maximumSizeElements'()
     ensures exists s :: s in Universe() && maximumSizeElements() == |s|*maximumSizeElements'()
 
-   ghost function {:axiom} maximumSizeElements'():nat
+  ghost function {:axiom} maximumSizeElements'():nat
     ensures forall s | s in Universe() :: (forall s' | s' in s :: maximumSizeElements'() >= |s'|*constant)
     ensures exists s | s in Universe() :: (exists s' | s' in s :: maximumSizeElements'() == |s'|*constant)
 
@@ -134,48 +165,55 @@ type SetSetSet< T(==) > {
     {|Universe()|*maximumSizeElements()}
 
   method {:axiom} Pick(ghost counter_in:nat) returns (e:SetSet<T>, ghost counter_out:nat)
+    requires Valid()
+    ensures e.Valid()
     requires Model() != {}
     ensures e.maximumSizeElements() == maximumSizeElements'()
     ensures e.Model() in Model()
     ensures counter_out == counter_in + maximumSizeElements()
 
   method {:axiom} Empty(ghost counter_in:nat) returns (b: bool, ghost counter_out:nat)
+    requires Valid()
     ensures b == (Model() == {})
     ensures counter_out == counter_in + constant
   
   method {:axiom} Cardinality(ghost counter_in:nat) returns (size: int, ghost counter_out:nat)
+    requires Valid()
     ensures  size == |Model()|
     ensures counter_out == counter_in + constant
   
+  method {:axiom} Contains(e:SetSet<T>, ghost counter_in:nat) returns (b:bool, ghost counter_out:nat)
+    requires Valid()
+    ensures  b == (e.Model() in Model()) 
+    ensures counter_out == counter_in + Size()
+  
   method {:axiom} Add(e:SetSet<T>, ghost counter_in:nat) returns (R:SetSetSet<T>, ghost counter_out:nat)
-    ensures R.Model() <= R.Universe()
+    requires Valid()
+    ensures R.Valid()
     ensures R.Universe() == Universe() + {e.Model()}
     ensures R.maximumSizeElements() == maximumSizeElements()
-    //requires e.Model() in Universe()
     ensures  R.Model() == Model() + {e.Model()}
     ensures if e.Model() in Model() then |R.Model()| == |Model()|
             else |R.Model()| == |Model()| + constant
     ensures if e.Model() in Universe() then |R.Universe()| == |Universe()|
             else |R.Universe()| == |Universe()| + constant
-    ensures counter_out == counter_in + maximumSizeElements()
+    ensures counter_out == counter_in + Size()
 
   method {:axiom} Remove(e:SetSet<T>, ghost counter_in:nat) returns (R:SetSetSet<T>, ghost counter_out:nat)
-    ensures R.Model() <= R.Universe()
+    requires Valid()
+    ensures R.Valid()
     ensures R.Universe() == Universe()
     ensures R.maximumSizeElements() == maximumSizeElements()
     ensures  R.Model() == Model() - {e.Model()}
     ensures if e.Model() !in Model() then |R.Model()| == |Model()|
             else |R.Model()| == |Model()| - 1
     ensures counter_out == counter_in + Size()
-  
-  method {:axiom} Contains(e:SetSet<T>, ghost counter_in:nat) returns (b:bool, ghost counter_out:nat)
-    ensures  b == (e.Model() in Model()) 
-    ensures counter_out == counter_in + Size()
 
   method {:axiom} Copy(ghost counter_in:nat) returns (R:SetSetSet<T>, ghost counter_out:nat)
+    requires Valid()
+    ensures R.Valid()
     ensures R.Model() == Model()
     ensures R.Universe() == Model()
-    ensures R.Model() <= R.Universe()
     ensures R.maximumSizeElements() == maximumSizeElements()
     ensures R.maximumSizeElements'() == maximumSizeElements'()
     ensures counter_out == counter_in + Size()
@@ -222,33 +260,21 @@ ghost predicate init_SetSetSet(S:SetSetSet) {
     (S.Model() == S.Universe())
 }
 
-
-ghost predicate correct_Set(S:Set) {
-  (S.Model() <= S.Universe())
-}
-ghost predicate correct_SetSet(S:SetSet) {
-  (S.Model() <= S.Universe())
-}
-ghost predicate correct_SetSetSet(S:SetSetSet) {
-  (S.Model() <= S.Universe())
-}
-
-
 ghost predicate in_universe_Set(S:Set, U:Set) {
-  (S.Universe() <= U.Model()) &&
-  (S.Model() <= U.Model()) &&
-  (S.Universe() <= U.Universe())
+  S.Valid() &&
+  U.Valid() &&
+  (S.Universe() <= U.Model())
 }
 ghost predicate in_universe_SetSet(S:SetSet, U:SetSet) {
+  S.Valid() &&
+  U.Valid() &&
   (S.Universe() <= U.Model()) &&
-  (S.Model() <= U.Model()) &&
-  (S.Universe() <= U.Universe()) &&
   (S.maximumSizeElements() <= U.maximumSizeElements())
 }
 ghost predicate in_universe_SetSetSet(S:SetSetSet, U:SetSetSet) {
+  S.Valid() &&
+  U.Valid() &&
   (S.Universe() <= U.Model()) &&
-  (S.Model() <= U.Model()) &&
-  (S.Universe() <= U.Universe()) &&
   (S.maximumSizeElements() <= U.maximumSizeElements()) &&
   (S.maximumSizeElements'() <= U.maximumSizeElements'())
 }
